Change congruence lemmas of Fμ,ref,par
The case of lam and case expressions that before required the terms to be
well-typed now require terms to be closed.

Separated definition context and context refinement from soundness_binary file.

F_mu_ref_par/soundness_binary.v
@@ -1,4 +1,3 @@
-Require Import Coq.Logic.Eqdep_dec.
 Require Import iris.proofmode.invariants iris.proofmode.weakestpre
         iris.proofmode.tactics.
 Require Import iris.program_logic.hoare.
@@ -6,199 +5,96 @@ Require Import iris.program_logic.lifting.
 Require Import iris.algebra.auth iris.algebra.dec_agree iris.algebra.frac
         iris.algebra.upred_big_op.
 From iris_logrel.F_mu_ref_par Require Import lang typing rules_binary
-        rules logrel_binary fundamental_binary.
+        rules logrel_binary fundamental_binary context_refinement.
 Require Import iris.program_logic.adequacy.
 Import uPred.
-
-Inductive context_item : Type :=
-| CTX_Lam
-| CTX_AppL (e2 : expr)
-| CTX_AppR (e1 : expr)
-(* Products *)
-| CTX_PairL (e2 : expr)
-| CTX_PairR (e1 : expr)
-| CTX_Fst
-| CTX_Snd
-(* Sums *)
-| CTX_InjL
-| CTX_InjR
-| CTX_CaseL (e1 : expr) (e2 : expr)
-| CTX_CaseM (e0 : expr) (e2 : expr)
-| CTX_CaseR (e0 : expr) (e1 : expr)
-(* Nat bin op *)
-| CTX_NBOPL (op : NatBinOP) (e2 : expr)
-| CTX_NBOPR (op : NatBinOP) (e1 : expr)
-(* If *)
-| CTX_IfL (e1 : expr) (e2 : expr)
-| CTX_IfM (e0 : expr) (e2 : expr)
-| CTX_IfR (e0 : expr) (e1 : expr)
-(* Recursive Types *)
-| CTX_Fold
-| CTX_Unfold
-(* Polymorphic Types *)
-| CTX_TLam
-| CTX_TApp
-(* Concurrency *)
-| CTX_Fork
-(* Reference Types *)
-| CTX_Alloc
-| CTX_Load
-| CTX_StoreL (e2 : expr)
-| CTX_StoreR (e1 : expr)
-(* Compare and swap used for fine-grained concurrency *)
-| CTX_CAS_L (e1 : expr) (e2 : expr)
-| CTX_CAS_M (e0 : expr) (e2 : expr)
-| CTX_CAS_R (e0 : expr) (e1 : expr).
-
-Fixpoint fill_ctx_item (ctx : context_item) (e : expr) : expr :=
-  match ctx with
-  | CTX_Lam => Lam e
-  | CTX_AppL e2 => App e e2
-  | CTX_AppR e1 => App e1 e
-  | CTX_PairL e2 => Pair e e2
-  | CTX_PairR e1 => Pair e1 e
-  | CTX_Fst => Fst e
-  | CTX_Snd => Snd e
-  | CTX_InjL => InjL e
-  | CTX_InjR => InjR e
-  | CTX_CaseL e1 e2 => Case e e1 e2
-  | CTX_CaseM e0 e2 => Case e0 e e2
-  | CTX_CaseR e0 e1 => Case e0 e1 e
-  | CTX_NBOPL op e2 => NBOP op e e2
-  | CTX_NBOPR op e1 => NBOP op e1 e
-  | CTX_IfL e1 e2 => If e e1 e2
-  | CTX_IfM e0 e2 => If e0 e e2
-  | CTX_IfR e0 e1 => If e0 e1 e
-  | CTX_Fold => Fold e
-  | CTX_Unfold => Unfold e
-  | CTX_TLam => TLam e
-  | CTX_TApp => TApp e
-  | CTX_Fork => Fork e
-  | CTX_Alloc => Alloc e
-  | CTX_Load => Load e
-  | CTX_StoreL e2 => Store e e2
-  | CTX_StoreR e1 => Store e1 e
-  | CTX_CAS_L e1 e2 => CAS e e1 e2
-  | CTX_CAS_M e0 e2 => CAS e0 e e2
-  | CTX_CAS_R e0 e1 => CAS e0 e1 e
-  end.
-
-Definition context := list context_item.
-
-Definition fill_ctx K e := foldr fill_ctx_item e K.
-
-Local Open Scope bin_logrel_scope.
-
-(** typed context *)
-Inductive typed_context_item :
-  context_item → (list type) → type → (list type) → type → Prop :=
-| TP_CTX_Lam : ∀ Γ τ τ',
-    typed_context_item CTX_Lam (TArrow τ τ' :: τ :: Γ) τ' Γ (TArrow τ τ')
-| TP_CTX_AppL (e2 : expr) : ∀ Γ τ τ',
-    typed Γ e2 τ →
-    typed_context_item (CTX_AppL e2) Γ (TArrow τ τ') Γ τ'
-| TP_CTX_AppR (e1 : expr) : ∀ Γ τ τ',
-    typed Γ e1 (TArrow τ τ') →
-    typed_context_item (CTX_AppR e1) Γ τ Γ τ'
-| TP_CTX_PairL (e2 : expr) : ∀ Γ τ τ',
-    typed Γ e2 τ' →
-    typed_context_item (CTX_PairL e2) Γ τ Γ (TProd τ τ')
-| TP_CTX_PairR (e1 : expr) : ∀ Γ τ τ',
-    typed Γ e1 τ →
-    typed_context_item (CTX_PairR e1) Γ τ' Γ (TProd τ τ')
-| TP_CTX_Fst : ∀ Γ τ τ',
-    typed_context_item CTX_Fst Γ (TProd τ τ') Γ τ
-| TP_CTX_Snd : ∀ Γ τ τ',
-    typed_context_item CTX_Snd Γ (TProd τ τ') Γ τ'
-| TP_CTX_InjL : ∀ Γ τ τ',
-    typed_context_item CTX_InjL Γ τ Γ (TSum τ τ')
-| TP_CTX_InjR : ∀ Γ τ τ',
-    typed_context_item CTX_InjR Γ τ' Γ (TSum τ τ')
-| TP_CTX_CaseL (e1 : expr) (e2 : expr) : ∀ Γ τ1 τ2 τ',
-    typed (τ1 :: Γ) e1 τ' → typed (τ2 :: Γ) e2 τ' →
-    typed_context_item (CTX_CaseL e1 e2) Γ (TSum τ1 τ2) Γ τ'
-| TP_CTX_CaseM (e0 : expr) (e2 : expr) : ∀ Γ τ1 τ2 τ',
-    typed Γ e0 (TSum τ1 τ2) → typed (τ2 :: Γ) e2 τ' →
-    typed_context_item (CTX_CaseM e0 e2) (τ1 :: Γ) τ' Γ τ'
-| TP_CTX_CaseR (e0 : expr) (e1 : expr) : ∀ Γ τ1 τ2 τ',
-    typed Γ e0 (TSum τ1 τ2) → typed (τ1 :: Γ) e1 τ' →
-    typed_context_item (CTX_CaseR e0 e1) (τ2 :: Γ) τ' Γ τ'
-| TP_CTX_IfL (e1 : expr) (e2 : expr) : ∀ Γ τ,
-    typed Γ e1 τ → typed Γ e2 τ →
-    typed_context_item (CTX_IfL e1 e2) Γ (TBool) Γ τ
-| TP_CTX_IfM (e0 : expr) (e2 : expr) : ∀ Γ τ,
-    typed Γ e0 (TBool) → typed Γ e2 τ →
-    typed_context_item (CTX_IfM e0 e2) Γ τ Γ τ
-| TP_CTX_IfR (e0 : expr) (e1 : expr) : ∀ Γ τ,
-    typed Γ e0 (TBool) → typed Γ e1 τ →
-    typed_context_item (CTX_IfR e0 e1) Γ τ Γ τ
-| TP_CTX_NBOPL op (e2 : expr) : ∀ Γ,
-    typed Γ e2 TNat →
-    typed_context_item (CTX_NBOPL op e2) Γ TNat Γ (NatBinOP_res_type op)
-| TP_CTX_NBOPR op (e1 : expr) : ∀ Γ,
-    typed Γ e1 TNat →
-    typed_context_item (CTX_NBOPR op e1) Γ TNat Γ (NatBinOP_res_type op)
-| TP_CTX_Fold : ∀ Γ τ,
-    typed_context_item CTX_Fold Γ τ.[(TRec τ)/] Γ (TRec τ)
-| TP_CTX_Unfold : ∀ Γ τ,
-    typed_context_item CTX_Unfold Γ (TRec τ) Γ τ.[(TRec τ)/]
-| TP_CTX_TLam : ∀ Γ τ,
-    typed_context_item
-      CTX_TLam (map (λ t : type, t.[ren (+1)]) Γ) τ Γ (TForall τ)
-| TP_CTX_TApp : ∀ Γ τ τ',
-    typed_context_item CTX_TApp Γ (TForall τ) Γ τ.[τ'/]
-| TP_CTX_Fork : ∀ Γ,
-    typed_context_item CTX_Fork Γ TUnit Γ TUnit
-| TPCTX_Alloc : ∀ Γ τ,
-    typed_context_item CTX_Alloc Γ τ Γ (Tref τ)
-| TP_CTX_Load : ∀ Γ τ,
-    typed_context_item CTX_Load Γ (Tref τ) Γ τ
-| TP_CTX_StoreL (e2 : expr) : ∀ Γ τ,
-    typed Γ e2 τ →
-    typed_context_item (CTX_StoreL e2) Γ (Tref τ) Γ TUnit
-| TP_CTX_StoreR (e1 : expr) : ∀ Γ τ,
-    typed Γ e1 (Tref τ) →
-    typed_context_item (CTX_StoreR e1) Γ τ Γ TUnit
-| TP_CTX_CasL (e1 : expr)  (e2 : expr) : ∀ Γ τ,
-    EqType τ → typed Γ e1 τ → typed Γ e2 τ →
-    typed_context_item (CTX_CAS_L e1 e2) Γ (Tref τ) Γ TBool
-| TP_CTX_CasM (e0 : expr) (e2 : expr) : ∀ Γ τ,
-    EqType τ → typed Γ e0 (Tref τ) → typed Γ e2 τ →
-    typed_context_item (CTX_CAS_M e0 e2) Γ τ Γ TBool
-| TP_CTX_CasR (e0 : expr) (e1 : expr) : ∀ Γ τ,
-    EqType τ → typed Γ e0 (Tref τ) → typed Γ e1 τ →
-    typed_context_item (CTX_CAS_R e0 e1) Γ τ Γ TBool.
-
-Lemma typed_context_item_typed k Γ τ Γ' τ' e :
-  typed Γ e τ → typed_context_item k Γ τ Γ' τ' →
-  typed Γ' (fill_ctx_item k e) τ'.
-Proof. intros H1 H2; induction H2; simpl; eauto using typed. Qed.
-
-Inductive typed_context :
-  context → (list type) → type → (list type) → type → Prop :=
-| TPCTX_nil : ∀ Γ τ, typed_context nil Γ τ Γ τ
-| TPCTX_cons : ∀ Γ1 τ1 Γ2 τ2 Γ3 τ3 k K,
-    typed_context_item k Γ2 τ2 Γ3 τ3 →
-    typed_context K Γ1 τ1 Γ2 τ2 →
-    typed_context (k :: K) Γ1 τ1 Γ3 τ3.
-
-Lemma typed_context_typed K Γ τ Γ' τ' e :
-  typed Γ e τ → typed_context K Γ τ Γ' τ' → typed Γ' (fill_ctx K e) τ'.
-Proof.
-  intros H1 H2; induction H2; simpl; eauto using typed_context_item_typed.
-Qed.
-
-Definition context_refines Γ e e' τ (He : typed Γ e τ) (He' : typed Γ e' τ) :=
-  ∀ K,
-    typed_context K Γ τ [] TUnit →
-    ∀ thp h v, rtc step ([fill_ctx K e], ∅) ((# v) :: thp, h) →
-               ∃ thp' h' v',
-                 rtc step ([fill_ctx K e'], ∅) ((# v') :: thp', h').
 
 Section Soundness.
   Context {Σ : gFunctors}
           {iI : heapIG Σ} {iS : cfgSG Σ}
           {N : namespace}.
+
+  Lemma bin_log_related_under_typed_context Γ e e' τ Γ' τ' K :
+    (∀ f, e.[iter (List.length Γ) up f] = e) →
+    (∀ f, e'.[iter (List.length Γ) up f] = e') →
+    typed_context K Γ τ Γ' τ' →
+    (∀ Δ {HΔ : context_interp_Persistent Δ},
+        @bin_log_related _ _ _ N Δ Γ e e' τ HΔ) →
+    ∀ Δ {HΔ : context_interp_Persistent Δ},
+      @bin_log_related _ _ _ N Δ Γ' (fill_ctx K e) (fill_ctx K e') τ' HΔ.
+  Proof.
+    revert Γ τ Γ' τ' e e'.
+    induction K as [|k K]=> Γ τ Γ' τ' e e' H1 H2; simpl.
+    - inversion_clear 1; trivial.
+    - inversion_clear 1 as [|? ? ? ? ? ? ? ? Hx1 Hx2]. intros H3 Δ HΔ.
+      specialize (IHK _ _ _ _ e e' H1 H2 Hx2 H3).
+      inversion Hx1; subst; simpl.
+      + eapply typed_binary_interp_Lam; eauto;
+          match goal with
+            H : _ |- _ => eapply (typed_context_n_closed _ _ _ _ _ _ _ H)
+          end.
+      + eapply typed_binary_interp_App; eauto using typed_binary_interp.
+      + eapply typed_binary_interp_App; eauto using typed_binary_interp.
+      + eapply typed_binary_interp_Pair; eauto using typed_binary_interp.
+      + eapply typed_binary_interp_Pair; eauto using typed_binary_interp.
+      + eapply typed_binary_interp_Fst; eauto.
+      + eapply typed_binary_interp_Snd; eauto.
+      + eapply typed_binary_interp_InjL; eauto.
+      + eapply typed_binary_interp_InjR; eauto.
+      + match goal with
+          H : typed_context_item _ _ _ _ _ |- _ => inversion H; subst
+        end.
+        eapply typed_binary_interp_Case;
+          eauto using typed_binary_interp;
+          match goal with
+            H : _ |- _ => eapply (typed_n_closed _ _ _ H)
+          end.
+      + match goal with
+          H : typed_context_item _ _ _ _ _ |- _ => inversion H; subst
+        end.
+        eapply typed_binary_interp_Case;
+          eauto using typed_binary_interp;
+          try match goal with
+                H : _ |- _ => eapply (typed_n_closed _ _ _ H)
+              end;
+          match goal with
+            H : _ |- _ => eapply (typed_context_n_closed _ _ _ _ _ _ _ H)
+          end.
+      + match goal with
+          H : typed_context_item _ _ _ _ _ |- _ => inversion H; subst
+        end.
+        eapply typed_binary_interp_Case;
+          eauto using typed_binary_interp;
+          try match goal with
+                H : _ |- _ => eapply (typed_n_closed _ _ _ H)
+              end;
+          match goal with
+            H : _ |- _ => eapply (typed_context_n_closed _ _ _ _ _ _ _ H)
+          end.
+      + eapply typed_binary_interp_If;
+          eauto using typed_context_typed, typed_binary_interp.
+      + eapply typed_binary_interp_If;
+          eauto using typed_context_typed, typed_binary_interp.
+      + eapply typed_binary_interp_If;
+          eauto using typed_context_typed, typed_binary_interp.
+      + eapply typed_binary_interp_nat_bin_op;
+          eauto using typed_context_typed, typed_binary_interp.
+      + eapply typed_binary_interp_nat_bin_op;
+          eauto using typed_context_typed, typed_binary_interp.
+      + eapply typed_binary_interp_Fold; eauto.
+      + eapply typed_binary_interp_Unfold; eauto.
+      + eapply typed_binary_interp_TLam; eauto.
+      + eapply typed_binary_interp_TApp; trivial.
+      + eapply typed_binary_interp_Fork; trivial.
+      + eapply typed_binary_interp_Alloc; trivial.
+      + eapply typed_binary_interp_Load; trivial.
+      + eapply typed_binary_interp_Store; eauto using typed_binary_interp.
+      + eapply typed_binary_interp_Store; eauto using typed_binary_interp.
+      + eapply typed_binary_interp_CAS; eauto using typed_binary_interp.
+      + eapply typed_binary_interp_CAS; eauto using typed_binary_interp.
+      + eapply typed_binary_interp_CAS; eauto using typed_binary_interp.
+        Unshelve. all: trivial.
+  Qed.
 
   Definition free_type_context : varC -n> bivalC -n> iPropG lang Σ :=
     {| cofe_mor_car := λ x, {| cofe_mor_car := λ y, (True)%I |} |}.
@@ -242,9 +138,6 @@ Section Soundness.
       inversion Hx1 as [|? ? Hx]; subst.
       apply frac_valid_inv_l in Hx. inversion Hx.
   Qed.
-
-  Lemma of_empty_heap : of_heap ∅ = ∅.
-  Proof. unfold of_heap; apply map_eq => i; rewrite !lookup_omap; f_equal. Qed.
 
   Local Arguments of_heap : simpl never.
 
@@ -295,66 +188,14 @@ Section Soundness.
           auth.auth_own. iFrame "Hheap Hspec Hg2"; trivial.
   Admitted.
 
-  Lemma bin_log_related_under_typed_context Γ e e' τ Γ' τ' K :
-    typed Γ e τ → typed Γ e' τ →
-    typed_context K Γ τ Γ' τ' →
+  Lemma Binary_Soundness Γ e e' τ :
+    (∀ f, e.[iter (List.length Γ) up f] = e) →
+    (∀ f, e'.[iter (List.length Γ) up f] = e') →
     (∀ Δ {HΔ : context_interp_Persistent Δ},
         @bin_log_related _ _ _ N Δ Γ e e' τ HΔ) →
-    ∀ Δ {HΔ : context_interp_Persistent Δ},
-      @bin_log_related _ _ _ N Δ Γ' (fill_ctx K e) (fill_ctx K e') τ' HΔ.
+    context_refines Γ e e' τ.
   Proof.
-    revert Γ τ Γ' τ' e e'.
-    induction K as [|k K]=> Γ τ Γ' τ' e e' H1 H2; simpl.
-    - inversion_clear 1; trivial.
-    - inversion_clear 1 as [|? ? ? ? ? ? ? ? Hx1 Hx2]. intros H3 Δ HΔ.
-      specialize (IHK _ _ _ _ e e' H1 H2 Hx2 H3).
-      inversion Hx1; subst; simpl.
-      + eapply typed_binary_interp_Lam; eauto using typed_context_typed.
-      + eapply typed_binary_interp_App; eauto using typed_binary_interp.
-      + eapply typed_binary_interp_App; eauto using typed_binary_interp.
-      + eapply typed_binary_interp_Pair; eauto using typed_binary_interp.
-      + eapply typed_binary_interp_Pair; eauto using typed_binary_interp.
-      + eapply typed_binary_interp_Fst; eauto.
-      + eapply typed_binary_interp_Snd; eauto.
-      + eapply typed_binary_interp_InjL; eauto.
-      + eapply typed_binary_interp_InjR; eauto.
-      + eapply typed_binary_interp_Case;
-          eauto using typed_context_typed, typed_binary_interp.
-      + eapply typed_binary_interp_Case;
-          eauto using typed_context_typed, typed_binary_interp.
-      + eapply typed_binary_interp_Case;
-          eauto using typed_context_typed, typed_binary_interp.
-      + eapply typed_binary_interp_If;
-          eauto using typed_context_typed, typed_binary_interp.
-      + eapply typed_binary_interp_If;
-          eauto using typed_context_typed, typed_binary_interp.
-      + eapply typed_binary_interp_If;
-          eauto using typed_context_typed, typed_binary_interp.
-      + eapply typed_binary_interp_nat_bin_op;
-          eauto using typed_context_typed, typed_binary_interp.
-      + eapply typed_binary_interp_nat_bin_op;
-          eauto using typed_context_typed, typed_binary_interp.
-      + eapply typed_binary_interp_Fold; eauto.
-      + eapply typed_binary_interp_Unfold; eauto.
-      + eapply typed_binary_interp_TLam; eauto.
-      + eapply typed_binary_interp_TApp; trivial.
-      + eapply typed_binary_interp_Fork; trivial.
-      + eapply typed_binary_interp_Alloc; trivial.
-      + eapply typed_binary_interp_Load; trivial.
-      + eapply typed_binary_interp_Store; eauto using typed_binary_interp.
-      + eapply typed_binary_interp_Store; eauto using typed_binary_interp.
-      + eapply typed_binary_interp_CAS; eauto using typed_binary_interp.
-      + eapply typed_binary_interp_CAS; eauto using typed_binary_interp.
-      + eapply typed_binary_interp_CAS; eauto using typed_binary_interp.
-  Qed.
-
-  Lemma Binary_Soundness Γ e e' τ
-        (He : typed Γ e τ) (He' : typed Γ e' τ) :
-    (∀ Δ {HΔ : context_interp_Persistent Δ},
-        @bin_log_related _ _ _ N Δ Γ e e' τ HΔ) →
-    context_refines Γ e e' τ He He'.
-  Proof.
-    intros H1 K HK htp hp v Hstp.
+    intros H1 K HK htp hp v Hstp Hc Hc'.
     eapply basic_soundness; eauto.
     eapply bin_log_related_under_typed_context; eauto.
   Qed.
